theories/L2k_noCnstrParams/stripEvalCommute.v
@@ -7,49 +7,48 @@ Require Import Coq.Arith.Peano_dec.
 Require Import Coq.Setoids.Setoid.
 Require Import Omega.
 
-Require Import L1g.L1g.
-Require Import L2.compile.
-Require Import L2.term.
-Require Import L2.program.
-Require Import L2.wndEval.
-Require Import L2.wcbvEval.
+Require Import L2.L2.
+Require Import L2k.compile.
+Require Import L2k.term.
+Require Import L2k.program.
+Require Import L2k.wcbvEval.
 
 Local Open Scope string_scope.
 Local Open Scope bool.
 Local Open Scope list.
 Set Implicit Arguments.
 
-Definition L1gTerm := L1g.compile.Term.
-Definition L1gTerms := L1g.compile.Terms.
-Definition L1gDefs := L1g.compile.Defs.
+Definition L1gTerm := L2.compile.Term.
+Definition L1gTerms := L2.compile.Terms.
+Definition L1gDefs := L2.compile.Defs.
 
 
-Definition optStrip (t:option L1gTerm) : option Term :=
+Definition optStrip (t:option L2Term) : option Term :=
   match t with
     | None => None
     | Some t => Some (strip t)
   end.
-Definition optStrips (ts:option L1gTerms) : option Terms :=
+Definition optStrips (ts:option L2Terms) : option Terms :=
   match ts with
     | None => None
     | Some ts => Some (strips ts)
   end.
-Definition optStripDnth (b: option (L1gTerm * nat)) : option (Term * nat) :=
+Definition optStripDnth (b: option (L2Term * nat)) : option (Term * nat) :=
                            match b with
                              | None => None
                              | Some (t, n) => Some (strip t, n)
                            end.
 Definition optStripCanP
-           (b: option (nat * L1gTerms)): option (nat * Terms) :=
+           (b: option (nat * L2Terms * nat)): option (nat * Terms * nat) :=
                            match b with
                              | None => None
-                             | Some (n, t) => Some (n, strips t)
+                             | Some (n, t, m) => Some (n, strips t, m)
                            end.
 Definition optStrip_split
-           (b: option L1g.term.split): option split :=
+           (b: option L2.term.split): option split :=
   match b with
     | None => None
-    | Some (L1g.term.mkSplit fsts t lsts) =>
+    | Some (L2.term.mkSplit fsts t lsts) =>
       Some (mkSplit (strips fsts) (strip t) (strips lsts))
   end.
 
@@ -57,7 +56,7 @@ Definition optStrip_split
 Lemma optStrip_hom: forall y, optStrip (Some y) = Some (strip y).
 induction y; simpl; reflexivity.
 Qed.
-Lemma optStrip_hom_None: optStrip (@None L1g.compile.Term) = @None (Term).
+Lemma optStrip_hom_None: optStrip (@None L2.compile.Term) = @None (Term).
   reflexivity.
 Qed.
 
@@ -69,19 +68,19 @@ Lemma optStripDnth_hom:
 induction y; simpl; reflexivity.
 Qed.
 Lemma optStripCanP_hom:
-  forall y n, optStripCanP (Some (n, y)) = Some (n, strips y).
+  forall y n m, optStripCanP (Some (n, y, m)) = Some (n, strips y, m).
 induction y; simpl; reflexivity.
 Qed.
 Lemma optStrip_split_hom:
   forall fsts t lsts,
-    optStrip_split (Some (L1g.term.mkSplit fsts t lsts)) =
+    optStrip_split (Some (L2.term.mkSplit fsts t lsts)) =
     Some (mkSplit (strips fsts) (strip t) (strips lsts)).
 Proof.
   induction fsts; cbn; intros; try reflexivity.
 Qed.
                               
 Lemma tlength_hom:
-  forall ts, tlength (strips ts) = L1g.term.tlength ts.
+  forall ts, tlength (strips ts) = L2.term.tlength ts.
 Proof.
   induction ts; intros; try reflexivity.
   - cbn. apply f_equal. assumption.
@@ -148,32 +147,32 @@ Proof.
 Qed.
 
 Lemma dlength_hom:
-  forall ds, L1g.compile.dlength ds = dlength (stripDs ds).
+  forall ds, L2.term.dlength ds = dlength (stripDs ds).
 induction ds. intuition. simpl. rewrite IHds. reflexivity.
 Qed.
 
 Lemma tcons_hom:
-  forall t ts, strips (L1g.compile.tcons t ts) = tcons (strip t) (strips ts).
+  forall t ts, strips (L2.compile.tcons t ts) = tcons (strip t) (strips ts).
 reflexivity.
 Qed.
 
-Lemma tnil_hom: strips L1g.compile.tnil = tnil.
+Lemma tnil_hom: strips L2.compile.tnil = tnil.
 reflexivity.
 Qed.
 
 Lemma dcons_hom:
-  forall nm ty bod rarg ds,
-    stripDs (L1g.compile.dcons nm ty bod rarg ds) =
+  forall nm bod rarg ds,
+    stripDs (L2.compile.dcons nm bod rarg ds) =
     dcons nm (strip bod) rarg (stripDs ds).
 reflexivity.
 Qed.
 
-Lemma dnil_hom: stripDs L1g.compile.dnil = dnil.
+Lemma dnil_hom: stripDs L2.compile.dnil = dnil.
 reflexivity.
 Qed.
 
 Lemma dnthBody_hom: 
-  forall m ds, optStripDnth (L1g.compile.dnthBody m ds) =
+  forall m ds, optStripDnth (L2.term.dnthBody m ds) =
                dnthBody m (stripDs ds).
 induction m; induction ds; try intuition.
 - simpl. intuition.
@@ -181,90 +180,123 @@ Qed.
 
 
 Lemma TCast_hom:
-  forall tm ty, strip (L1g.compile.TCast tm ty) = TCast (strip tm).
+  forall tm, strip (L2.compile.TCast tm) = TCast (strip tm).
 Proof.
   reflexivity.
 Qed.
 
+(****
 Lemma canonicalP_hom:
-  forall t, optStripCanP (L1g.term.canonicalP t) = canonicalP (strip t).
+  forall t, optStripCanP (L2.term.canonicalP t) = canonicalP (strip t).
 Proof.
   destruct t; intros; cbn; try reflexivity.
   destruct t1; cbn; try reflexivity.
 Qed.
+ ****)
 
 Lemma tnth_hom:
- forall ts n, optStrip (L1g.term.tnth n ts) = tnth n (strips ts).
+ forall ts n, optStrip (L2.term.tnth n ts) = tnth n (strips ts).
 induction ts; simpl; intros n; case n; try reflexivity; trivial.
 Qed. 
 
 Lemma tskipn_hom:
-  forall ts n, optStrips (L1g.term.tskipn n ts) = tskipn n (strips ts).
+  forall ts n, optStrips (L2.term.tskipn n ts) = tskipn n (strips ts).
 induction ts; simpl; intros n; case n; try reflexivity; trivial.
 Qed.
 
 Lemma tappend_hom:
   forall ts us,
-    strips (L1g.compile.tappend ts us) = tappend (strips ts) (strips us).
-induction ts; intros us; simpl. reflexivity.
-rewrite IHts. reflexivity.
+    strips (L2.term.tappend ts us) = tappend (strips ts) (strips us).
+Proof.
+  induction ts; intros us; simpl. reflexivity.
+  rewrite IHts. reflexivity.
 Qed.
 
 Lemma TApp_hom:
-  forall fn arg args,
-    strip (L1g.compile.TApp fn arg args) =
+  forall fn arg args, ~ L2.term.isConstruct fn ->
+    strip (L2.compile.TApp fn arg args) =
     TApp (strip fn) (strip arg) (strips args).
-induction fn; intros arg args; try reflexivity.
+Proof.
+  destruct fn; intros arg args h; try reflexivity.
+  elim h. auto.
 Qed.
 
 Lemma isApp_hom:
-  forall t, isApp (strip t) -> L1g.term.isApp t.
+  forall t,
+    isApp (strip t) -> L2.term.isApp t.
 Proof.
-  destruct t; simpl; intros h;
-  destruct h as [x0 [x1 [x2 h]]]; try discriminate. 
-  exists t1, t2, t3. reflexivity.
+  destruct t; cbn; intros h;
+  destruct h as [x0 [x1 [x2 h]]]; try discriminate; auto.     
+  - destruct (etaExp_cnstr_Sanity' i n n0 n1 tnil).
+    + rewrite h in H. destruct H as [y0 [y1 [y2 jy]]]. discriminate.
+    + rewrite h in H. destruct H as [y0 [y1 jy]]. discriminate.
+  - destruct p. discriminate.
 Qed.
 
 Lemma isLambda_hom:
-  forall t, isLambda (strip t) -> L1g.term.isLambda t.
+  forall t,
+    isLambda (strip t) ->
+    L2.term.isLambda t \/ L2.term.isConstruct t \/  L2.term.isApp t.
 Proof.
-  destruct t; simpl; intros h; destruct h as [x0 [x1 h]]; try discriminate. 
-  exists n, t1, t2. reflexivity.
+  intros t. functional induction (strip t); intros h;
+  destruct h as [x0 [x1 jx]]; try discriminate.
+  - left. auto.
+  - right. right. auto.
+  - right. left. auto.
 Qed.
 
 Lemma isFix_hom:
-  forall t, isFix (strip t) -> L1g.term.isFix t.
+  forall t, isFix (strip t) -> L2.term.isFix t.
 Proof.
-  destruct t; cbn; intros h; destruct h as [x0 [x1 h]]; try discriminate.
-  exists d, n. reflexivity. 
+  induction t; intros; cbn in *;
+  try (destruct H as [x0 [x1 jx]]; discriminate); auto.
+  - destruct t1; try (destruct H as [x0 [x1 jx]]; discriminate).
+    assert (j:= etaExp_cnstr_sanity i n n0 n1 (tcons (strip t2) (strips t3))).
+    destruct (n0 + n1 - tlength (tcons (strip t2) (strips t3))).
+    + destruct j as [x0 [x1 [x2 jx]]]. rewrite jx in H.
+      destruct H as [y0 [y1 jy]]. discriminate.
+    + destruct j as [x0 [x1 jx]]. rewrite jx in H.
+      destruct H as [y0 [y1 jy]]. discriminate.
+  - assert (j:= etaExp_cnstr_sanity i n n0 n1 tnil).
+    destruct (n0 + n1); cbn in j.
+    + destruct j as [x0 [x1 [x2 jx]]]. rewrite jx in H.
+      destruct H as [y0 [y1 jy]]. discriminate.
+    + destruct j as [x0 [x1 jx]]. rewrite jx in H.
+      destruct H as [y0 [y1 jy]]. discriminate.
+  - destruct p. destruct H as [y0 [y1 jy]]. discriminate.
 Qed.
 
-Lemma L1WFapp_L2WFapp:
-  (forall t, L1g.term.WFapp t -> WFapp (strip t)) /\
-  (forall ts, L1g.term.WFapps ts -> WFapps (strips ts)) /\
-  (forall ds, L1g.term.WFappDs ds -> WFappDs (stripDs ds)).
+
+Lemma L2WFapp_L2kWFapp:
+  (forall t, L2.term.WFapp t -> WFapp (strip t)) /\
+  (forall ts, L2.term.WFapps ts -> WFapps (strips ts)) /\
+  (forall ds, L2.term.WFappDs ds -> WFappDs (stripDs ds)).
 Proof.
-  apply L1g.term.WFappTrmsDefs_ind; simpl; constructor; auto.
-  intros h. elim H. apply isApp_hom. assumption.
+  apply L2.term.WFappTrmsDefs_ind; cbn; try constructor; auto; intros.
+  - destruct fn; cbn; auto; try (constructor; try assumption; not_isApp).
+    + apply etaExp_cnstr_pres_WFapp. constructor; assumption.
+    + destruct p. constructor; try assumption. not_isApp.
+  - apply etaExp_cnstr_pres_WFapp. constructor.
+  - destruct m. constructor; try assumption.
 Qed.
 
-Lemma L1WFaEnv_L2WFaEnv:
-  forall p:environ L1gTerm, L1g.program.WFaEnv p -> WFaEnv (stripEnv p).
+Lemma L2WFaEnv_L2kWFaEnv:
+  forall p:environ L2Term, L2.program.WFaEnv p -> WFaEnv (stripEnv p).
 Proof.
   induction 1; simpl; constructor.
   - inversion H; destruct ec; simpl; try discriminate; constructor.
-    + apply (proj1 (L1WFapp_L2WFapp)). assumption.
+    + apply (proj1 (L2WFapp_L2kWFapp)). assumption.
   - assumption.
   - apply stripEnv_pres_fresh. assumption.
 Qed.
 
 (***
 Lemma WFapp_hom:
-  (forall t, L1g.term.WFapp t -> WFapp (strip t)) /\
-  (forall ts, L1g.term.WFapps ts -> WFapps (strips ts)) /\
-  (forall ds, L1g.term.WFappDs ds -> WFappDs (stripDs ds)).
+  (forall t, L2.term.WFapp t -> WFapp (strip t)) /\
+  (forall ts, L2.term.WFapps ts -> WFapps (strips ts)) /\
+  (forall ds, L2.term.WFappDs ds -> WFappDs (stripDs ds)).
 Proof.
-   apply L1g.term.WFappTrmsDefs_ind; cbn; intros;
+   apply L2.term.WFappTrmsDefs_ind; cbn; intros;
   try (solve [constructor]);
   try (solve [constructor; intuition]).
   - constructor; try assumption.
@@ -290,17 +322,45 @@ Proof.
   - rewrite mkApp_idempotent. simpl. reflexivity.
 Qed.
 
+(***
 Lemma mkApp_hom:
-forall fn args,
-  strip (L1g.term.mkApp fn args) = mkApp (strip fn) (strips args).
+forall fn args, ~ L2.term.isApp fn ->
+  strip (L2.term.mkApp fn args) = mkApp (strip fn) (strips args).
 Proof.
+  intros. destruct args.
+  - rewrite L2.term.mkApp_tnil_ident. rewrite mkApp_tnil_ident. reflexivity.
+  - rewrite L2.term.mkApp_goodFn; try assumption. rewrite tcons_hom.
+    assert (j: ~ isApp (strip fn)).
+    { intros h. elim H. apply isApp_hom. assumption. }
+    rewrite mkApp_goodFn; try assumption. destruct fn; cbn; try reflexivity.
+    unfold strip in j.
+    
   destruct args; try (reflexivity).
-  - rewrite L1g.term.mkApp_tnil_ident. rewrite mkApp_tnil_ident.
+  - rewrite L2.term.mkApp_tnil_ident. rewrite mkApp_tnil_ident.
     reflexivity.
-  - destruct fn; try reflexivity.
+  - destruct (L2.term.isApp_dec fn).
+    + admit.
+    + rewrite L2.term.mkApp_goodFn; try assumption.
+      destruct (L2.term.isConstruct_dec fn).
+      * { destruct H as [x0 [x1 [x2 [x3 jx]]]]. subst. cbn.
+          destruct (etaExp_cnstr_Sanity'
+                      x0 x1 x2 x3 (tcons (strip t) (strips args))).
+          - destruct H as [y0 [y1 [y2 jy]]]. rewrite jy.
+            destruct (etaExp_cnstr_Sanity' x0 x1 x2 x3 tnil).
+            + destruct H as [z0 [z1 [z2 jz]]]. rewrite jz. cbn. rewrite <- jy.
+
+
+
+              destruct (etaExp_cnstr_Sanity' x0 x1 x2 x3 tnil).
+          
+          assert (j:= etaExp_cnstr_Sanity
+                        x0 x1 x2 x3 (tcons (strip t) (strips args))).
+          rewrite TApp_hom. admit. ; try assumption.
+
+    case_eq fn; intros; try reflexivity.
     cbn. rewrite <- tcons_hom. rewrite <- tappend_hom. reflexivity.
 Qed.
-
+***)
 
 Lemma instantiate_tappend_commute:
   forall ts us tin n,
@@ -347,15 +407,16 @@ induction bod; simpl; intros; try reflexivity.
   reflexivity.
 Qed.
 
+(*****************  broken from here  ************
 Lemma instantiate_hom:
-  (forall bod arg n, strip (L1g.term.instantiate arg n bod) =
+  (forall bod arg n, strip (L2.term.instantiate arg n bod) =
                      instantiate (strip arg) n (strip bod)) /\
-    (forall bods arg n, strips (L1g.term.instantiates arg n bods) =
+  (forall bods arg n, strips (L2.term.instantiates arg n bods) =
                     instantiates (strip arg) n (strips bods)) /\
-    (forall ds arg n, stripDs (L1g.term.instantiateDefs arg n ds) =
-                      instantiateDefs (strip arg) n (stripDs ds)).
+  (forall ds arg n, stripDs (L2.term.instantiateDefs arg n ds) =
+                    instantiateDefs (strip arg) n (stripDs ds)).
 Proof.
-  apply L1g.compile.TrmTrmsDefs_ind; intros; try (simpl; reflexivity).
+  apply L2.compile.TrmTrmsDefs_ind; intros; try (simpl; reflexivity).
   - simpl. destruct (lt_eq_lt_dec n n0); cbn.
     + destruct s.
       * rewrite (proj1 (nat_compare_gt n0 n)); try omega. cbn. reflexivity.
@@ -363,50 +424,41 @@ Proof.
     + rewrite (proj1 (nat_compare_lt n0 n)); trivial.
   - cbn. rewrite H. reflexivity.
   - cbn. rewrite H. reflexivity.
-  - change (TProd n (strip (L1g.term.instantiate arg (S n0) t0)) =
-            (TProd n (instantiate (strip arg) (S n0) (strip t0)))).
-    rewrite H0. reflexivity.
-  - change (TLambda n (strip (L1g.term.instantiate arg (S n0) t0)) =
-            (TLambda n (instantiate (strip arg) (S n0) (strip t0)))).
-    rewrite H0. reflexivity.
-  - change (TLetIn n (strip (L1g.term.instantiate arg n0 t))
-                   (strip (L1g.term.instantiate arg (S n0) t1)) =
-            (TLetIn n (instantiate (strip arg) n0 (strip t))
-                    (instantiate (strip arg) (S n0) (strip t1)))).
-    rewrite H. rewrite H1. reflexivity.
-  - change (strip (L1g.term.mkApp
-                     (L1g.term.instantiate arg n t)
-                     (L1g.compile.tcons (L1g.term.instantiate arg n t0)
-                                         (L1g.term.instantiates arg n t1))) =
-            instantiate (strip arg) n (strip (L1g.compile.TApp t t0 t1))). 
+  - cbn. rewrite H. reflexivity.
+  - cbn. rewrite H. rewrite H0. reflexivity.
+  - change (strip (L2.term.mkApp
+                     (L2.term.instantiate arg n t)
+                     (L2.compile.tcons (L2.term.instantiate arg n t0)
+                                         (L2.term.instantiates arg n t1))) =
+            instantiate (strip arg) n (strip (L2.compile.TApp t t0 t1))). 
     rewrite TApp_hom. 
     change
-      (strip (L1g.term.mkApp
-                (L1g.term.instantiate arg n t)
-                (L1g.compile.tcons (L1g.term.instantiate arg n t0)
-                                   (L1g.term.instantiates arg n t1))) =
+      (strip (L2.term.mkApp
+                (L2.term.instantiate arg n t)
+                (L2.compile.tcons (L2.term.instantiate arg n t0)
+                                   (L2.term.instantiates arg n t1))) =
        (mkApp (instantiate (strip arg) n (strip t))
               (tcons (instantiate (strip arg) n (strip t0))
                      (instantiates (strip arg) n (strips t1))))).
     rewrite <- H. rewrite <- H0. rewrite <- H1. 
     rewrite mkApp_hom. rewrite tcons_hom. reflexivity.
-  - change (TCase p (strip (L1g.term.instantiate arg n t0))
-                  (stripDs (L1g.term.instantiateDefs arg n d)) =
+  - change (TCase p (strip (L2.term.instantiate arg n t0))
+                  (stripDs (L2.term.instantiateDefs arg n d)) =
             (TCase p (instantiate (strip arg) n (strip t0))
                    (instantiateDefs (strip arg) n (stripDs d)))).
     rewrite H0. rewrite H1. reflexivity.
-  - change (TFix (stripDs (L1g.term.instantiateDefs
-                             arg (n0 + L1g.compile.dlength d) d)) n =
+  - change (TFix (stripDs (L2.term.instantiateDefs
+                             arg (n0 + L2.compile.dlength d) d)) n =
             (TFix (instantiateDefs
                      (strip arg) (n0 + dlength (stripDs d)) (stripDs d)) n)).
     rewrite H. rewrite dlength_hom. reflexivity.
-  - change (tcons (strip (L1g.term.instantiate arg n t))
-                  (strips (L1g.term.instantiates arg n t0)) =
+  - change (tcons (strip (L2.term.instantiate arg n t))
+                  (strips (L2.term.instantiates arg n t0)) =
             tcons (instantiate (strip arg) n (strip t))
                   (instantiates (strip arg) n (strips t0))).
     rewrite H. rewrite H0. reflexivity.
-  - change (dcons n (strip (L1g.term.instantiate arg n1 t0)) n0
-                  (stripDs (L1g.term.instantiateDefs arg n1 d)) =
+  - change (dcons n (strip (L2.term.instantiate arg n1 t0)) n0
+                  (stripDs (L2.term.instantiateDefs arg n1 d)) =
             dcons n (instantiate (strip arg) n1 (strip t0)) n0
                   (instantiateDefs (strip arg) n1 (stripDs d))).
     rewrite H0. rewrite H1. reflexivity.
@@ -414,23 +466,24 @@ Qed.
 
 Lemma whBetaStep_hom:
   forall bod arg args,
-    strip (L1g.term.whBetaStep bod arg args) =
+    strip (L2.term.whBetaStep bod arg args) =
     whBetaStep (strip bod) (strip arg) (strips args).
 Proof.
   intros bod arg args.
-  unfold L1g.term.whBetaStep, whBetaStep.
+  unfold L2.term.whBetaStep, whBetaStep.
   rewrite mkApp_hom. rewrite <- (proj1 instantiate_hom). reflexivity.
 Qed.
 
+(***
 Lemma TConstruct_hom:
-  forall i n np na,
-    strip (L1g.compile.TConstruct i n np na) = TConstruct i n np na.
+  forall i n args,
+    strip (L2.compile.TConstruct i n args) = TConstruct i n args.
 intros. simpl.  destruct i. reflexivity.
 Qed.
-
+***)
 
 Lemma optStrip_match:
-  forall x (f:L1gTerm -> L1gTerm) (g:Term -> Term), 
+  forall x (f:L2Term -> L2Term) (g:Term -> Term), 
     (forall z, strip (f z) = g (strip z)) ->
     optStrip (match x with Some y => Some (f y) | None => None end) =
     match (optStrip x) with Some y => Some (g y) | None => None end.
@@ -441,51 +494,51 @@ Qed.
 
 Lemma whCaseStep_hom:
   forall n brs ts,
-    optStrip (L1g.term.whCaseStep n ts brs) =
+    optStrip (L2.term.whCaseStep n ts brs) =
     whCaseStep n (strips ts) (stripDs brs).
 destruct n, brs; intros; simpl; try reflexivity.
 - unfold whCaseStep. simpl. rewrite mkApp_hom. reflexivity.
-- unfold whCaseStep. unfold L1g.term.whCaseStep. cbn. 
+- unfold whCaseStep. unfold L2.term.whCaseStep. cbn. 
   rewrite <- dnthBody_hom. destruct (compile.dnthBody n brs); simpl.
   + destruct p as [x0 x1]. cbn. rewrite mkApp_hom. reflexivity.
   + reflexivity.
 Qed.
 
 Lemma TFix_hom:
-  forall defs n, strip (L1g.compile.TFix defs n) = TFix (stripDs defs) n.
+  forall defs n, strip (L2.compile.TFix defs n) = TFix (stripDs defs) n.
 reflexivity.
 Qed.
 
 Lemma TProd_hom:
   forall nm ty bod,
-    strip (L1g.compile.TProd nm ty bod) = TProd nm (strip bod).
+    strip (L2.compile.TProd nm ty bod) = TProd nm (strip bod).
 reflexivity.
 Qed.
 
 Lemma TLambda_hom:
   forall nm ty bod,
-    strip (L1g.compile.TLambda nm ty bod) = TLambda nm (strip bod).
+    strip (L2.compile.TLambda nm ty bod) = TLambda nm (strip bod).
 reflexivity.
 Qed.
 
 Lemma TLetIn_hom:
   forall nm dfn ty bod,
-    strip (L1g.compile.TLetIn nm dfn ty bod) =
+    strip (L2.compile.TLetIn nm dfn ty bod) =
     TLetIn nm (strip dfn) (strip bod).
 reflexivity.
 Qed.
 
 Lemma TCase_hom:
   forall n ty mch brs,
-    strip (L1g.compile.TCase n ty mch brs) =
+    strip (L2.compile.TCase n ty mch brs) =
     TCase n (strip mch) (stripDs brs).
 reflexivity.
 Qed.
 
 Lemma fold_left_hom:
-forall (F:L1gTerm -> nat -> L1gTerm) 
-       (stripF:Term -> nat -> Term) (ns:list nat) (t:L1gTerm),
-  (forall (s:L1gTerm) (n:nat), strip (F s n) = stripF (strip s) n) ->
+forall (F:L2Term -> nat -> L2Term) 
+       (stripF:Term -> nat -> Term) (ns:list nat) (t:L2Term),
+  (forall (s:L2Term) (n:nat), strip (F s n) = stripF (strip s) n) ->
   strip (fold_left F ns t) = fold_left stripF ns (strip t).
 induction ns; intros t h.
 - intuition.
@@ -497,16 +550,16 @@ Qed.
 Lemma pre_whFixStep_hom:
   forall body dts args,
     pre_whFixStep (strip body) (stripDs dts) (strips args) =
-    strip (L1g.term.pre_whFixStep body dts args).
+    strip (L2.term.pre_whFixStep body dts args).
 Proof.
   intros body dts args.
-  destruct dts, args; unfold pre_whFixStep, L1g.term.pre_whFixStep;
+  destruct dts, args; unfold pre_whFixStep, L2.term.pre_whFixStep;
   simpl; rewrite mkApp_hom; try reflexivity.
   - rewrite (fold_left_hom _
           (fun (bod : Term) (ndx : nat) =>
                 instantiate (TFix (dcons n (strip t0) n0 (stripDs dts)) ndx)
                   0 bod)).
-    + rewrite <- (dcons_hom _ L1g.compile.prop).
+    + rewrite <- (dcons_hom _ L2.compile.prop).
       rewrite (proj1 instantiate_hom).
       rewrite <- dlength_hom. reflexivity. 
     + intros. rewrite (proj1 instantiate_hom). simpl. reflexivity.
@@ -516,22 +569,22 @@ Proof.
     + rewrite dlength_hom. rewrite (proj1 instantiate_hom).
       rewrite tcons_hom. reflexivity.
     + intros. rewrite (proj1 instantiate_hom).
-      rewrite <- (dcons_hom _ L1g.compile.prop). simpl. reflexivity.
+      rewrite <- (dcons_hom _ L2.compile.prop). simpl. reflexivity.
 Qed.
 
 Lemma tsplit_hom:
   forall ix arg args,
-    optStrip_split (L1g.term.tsplit ix arg args) =
+    optStrip_split (L2.term.tsplit ix arg args) =
     tsplit ix (strip arg) (strips args).
 Proof.
   intros ix arg args.
-  functional induction (L1g.term.tsplit ix arg args); cbn; intros.
+  functional induction (L2.term.tsplit ix arg args); cbn; intros.
   - reflexivity.
   - destruct n. elim y. reflexivity.
   - destruct ls; cbn; reflexivity.
   - case_eq (tsplit m (strip t) (strips ts)); intros.
     + destruct s.
-      assert (j0:= L1g.term.tsplit_sanity m t ts). rewrite e1 in j0.
+      assert (j0:= L2.term.tsplit_sanity m t ts). rewrite e1 in j0.
       assert (j1:= tsplit_sanity m (strip t) (strips ts)).
       rewrite H in j1. destruct j1.
       assert (j2: tlength (strips ts) = tlength fsts + tlength lsts).
@@ -548,70 +601,19 @@ Qed.
 
 Lemma optStripCanP_hom':
   forall z, optStripCanP (Some z) =
-            Some (fst z, strips (snd z)).
-intros. destruct z as [z0 z1]. cbn. reflexivity.
+            Some (fst (fst z), strips (snd (fst z)), snd z).
+intros. destruct z as [[z0 z1] z2]. cbn. reflexivity.
 Qed.
 
-(***** Can this weaker version of WcbvEval_hom be proven?
-****  Seems need stronger IH   **************
-Lemma compile_pres_wcbvEval:
-  forall p,
-    (forall t t', L1g.wcbvEval.WcbvEval p t t' ->
-                  exists u, WcbvEval (stripEnv p) (strip t) u) /\
-    (forall ts ts', L1g.wcbvEval.WcbvEvals p ts ts' ->
-                  exists us, WcbvEvals (stripEnv p) (strips ts) us).
-Proof.
-  intros p.
-  apply L1g.wcbvEval.WcbvEvalEvals_ind; intros; cbn.
-  - destruct H as [x jx]. exists x. econstructor. assumption.
-  - destruct H as [x jx]. exists (TLambda nm (strip bod)). econstructor.
-  - destruct H as [x jx]. exists (TProd nm (strip bod)). econstructor.
-  - destruct H as [x jx]. exists x. constructor. assumption.
-  - exists (TConstruct i r arty). constructor.
-  - exists (TInd i). constructor.
-  - exists (TSort srt). constructor.
-  - exists (TFix (stripDs dts) m). constructor.
-  - exists TAx. constructor.
-  - destruct H as [x jx]. exists x. econstructor; try eassumption.
-    eapply (lookupDfn_hom _ _ e).
-  - destruct H as [x jx]. destruct H0 as [y jy]. destruct H1 as [z jz].
-    rewrite whBetaStep_hom in jz. exists z.
-    eapply (@wAppLam
-             (stripEnv p) (strip fn)
-             (strip bod) (strip a1) (strip a1') z (strips args) _ _ _ jz).
-  - destruct H as [x jx]. destruct H0 as [y jy].
-    rewrite (proj1 instantiate_hom) in jy. exists y.
-    eapply (@wLetIn (stripEnv p) nm (strip dfn) (strip bod) _ _ _ jy). 
-  - destruct H as [u ju]. destruct H0 as [y jy]. destruct H1 as [z jz].
-    rewrite <- pre_whFixStep_hom in jz. cbn in jy. cbn in jz. exists z.
-    eapply (@wAppFix
-             (stripEnv p) (stripDs dts) m
-             (strip fn) (strip arg) (strip arg') z (strip x)
-          (strips args) (strips args') ix _ _ _ _ jz).
-  - admit.
-  - admit.
-  - admit.
-  - admit.
-  - admit.
-  - admit.
-  - admit.
-    Grab Existential Variables.
-    rewrite tlength_hom. assumption.
-    rewrite <- dnthBody_hom. rewrite e. cbn. reflexivity.
-    admit.
-    admit.
-****)
-
-    
 Lemma WcbvEval_hom:
   forall p,
-    (forall t t', L1g.wcbvEval.WcbvEval p t t' ->
+    (forall t t', L2.wcbvEval.WcbvEval p t t' ->
                   WcbvEval (stripEnv p) (strip t) (strip t')) /\
-    (forall ts ts', L1g.wcbvEval.WcbvEvals p ts ts' ->
+    (forall ts ts', L2.wcbvEval.WcbvEvals p ts ts' ->
                     WcbvEvals (stripEnv p) (strips ts) (strips ts')).
 Proof.
   intros p.
-  apply L1g.wcbvEval.WcbvEvalEvals_ind; intros; try reflexivity;
+  apply L2.wcbvEval.WcbvEvalEvals_ind; intros; try reflexivity;
   try (solve[constructor; trivial]).
   - cbn. econstructor; try eassumption. apply lookupDfn_hom. assumption.
   - cbn. eapply wAppLam.
@@ -636,6 +638,9 @@ Proof.
     + rewrite <- dnthBody_hom. rewrite e. reflexivity.
     + rewrite tlength_hom. assumption. 
   - refine (wCase _ _ _ _ _ _ _); try eassumption.
+    +
+
+      
     * rewrite <- canonicalP_hom. rewrite e. reflexivity.
     * rewrite <- tskipn_hom. rewrite e0. reflexivity.
     * rewrite <- whCaseStep_hom. rewrite e1. reflexivity.
@@ -645,11 +650,11 @@ Qed.
 Print Assumptions WcbvEval_hom.
 
 (** WcbvEval_hom is nice, but it is stronger than necessary to prove 
-*** certiL1g_to_L2Correct (in instances.v).
+*** certiL2_to_L2Correct (in instances.v).
 **)
 Corollary strip_pres_eval:
-  forall (p:environ L1g.compile.Term) (t tv:L1g.compile.Term),
-    L1g.wcbvEval.WcbvEval p t tv ->
+  forall (p:environ L2.compile.Term) (t tv:L2.compile.Term),
+    L2.wcbvEval.WcbvEval p t tv ->
     exists stv, WcbvEval (stripEnv p) (strip t) stv.
 Proof.
   intros. exists (strip tv). apply (proj1 (WcbvEval_hom _)).
@@ -658,11 +663,11 @@ Qed.
 
 Corollary wcbvEval_hom:
   forall p n t t',
-    L1g.wcbvEval.wcbvEval p n t = Ret t' ->
+    L2.wcbvEval.wcbvEval p n t = Ret t' ->
     exists m, wcbvEval (stripEnv p) m (strip t) = Ret (strip t').
 Proof.
   intros. 
-  assert (j1:= proj1 (L1g.wcbvEval.wcbvEval_WcbvEval p n) _ _ H).
+  assert (j1:= proj1 (L2.wcbvEval.wcbvEval_WcbvEval p n) _ _ H).
   assert (k0:= proj1 (WcbvEval_hom p) _ _ j1).
   assert (j2:= @WcbvEval_wcbvEval (stripEnv p) (strip t) (strip t') k0).
   destruct j2 as [ny jny].
@@ -672,7 +677,7 @@ Qed.
 
 Lemma Prf_strip_inv:
   forall s st, TProof st = strip s ->
-              exists t, s = L1g.compile.TProof t /\ st = strip t.
+              exists t, s = L2.compile.TProof t /\ st = strip t.
 Proof.
   destruct s; simpl; intros h; try discriminate.
   intros. myInjection H. exists s. intuition.
@@ -681,7 +686,7 @@ Qed.
 Lemma Lam_strip_inv:
   forall nm bod s, TLambda nm bod = strip s ->
    exists sty sbod, 
-     (L1g.compile.TLambda nm sty sbod) = s /\ bod = strip sbod.
+     (L2.compile.TLambda nm sty sbod) = s /\ bod = strip sbod.
 Proof.
   intros nm bod; destruct s; simpl; intros h; try discriminate.
   - myInjection h. exists s1, s2. intuition. 
@@ -690,7 +695,7 @@ Qed.
 Lemma Prod_strip_inv:
   forall nm bod s, TProd nm bod = strip s ->
    exists sty sbod, 
-     (L1g.compile.TProd nm sty sbod) = s /\ bod = strip sbod.
+     (L2.compile.TProd nm sty sbod) = s /\ bod = strip sbod.
 Proof.
   intros nm bod; destruct s; simpl; intros h; try discriminate.
   - myInjection h. exists s1, s2. intuition. 
@@ -699,36 +704,36 @@ Qed.
 Lemma Cast_strip_inv:
   forall tm s, TCast tm = strip s ->
    exists stm sty, 
-     (L1g.compile.TCast stm sty) = s /\ tm = strip stm.
+     (L2.compile.TCast stm sty) = s /\ tm = strip stm.
 Proof.
   intros tm; destruct s; simpl; intros h; try discriminate.
   - myInjection h. exists s1, s2. intuition. 
 Qed.
 
 Lemma Construct_strip_inv:
-  forall i n np na s,
-    TConstruct i n np na = strip s -> L1g.compile.TConstruct i n np na = s.
+  forall i n arty s,
+    TConstruct i n arty = strip s -> L2.compile.TConstruct i n arty = s.
 Proof.
   intros i n. destruct s; simpl; intros h; try discriminate.
   - myInjection h. reflexivity.
 Qed.
 
 Lemma Sort_strip_inv:
-  forall srt s, TSort srt = strip s -> L1g.compile.TSort srt = s.
+  forall srt s, TSort srt = strip s -> L2.compile.TSort srt = s.
 Proof.
   intros srt. destruct s; simpl; intros h; try discriminate.
   - myInjection h. reflexivity.
 Qed.
 
 Lemma Ind_strip_inv:
-  forall i s, TInd i = strip s -> L1g.compile.TInd i = s.
+  forall i s, TInd i = strip s -> L2.compile.TInd i = s.
 Proof.
   intros i. destruct s; simpl; intros h; try discriminate.
   - myInjection h. reflexivity.
 Qed.
 
 Lemma Const_strip_inv:
-  forall nm s, TConst nm = strip s -> L1g.compile.TConst nm = s.
+  forall nm s, TConst nm = strip s -> L2.compile.TConst nm = s.
 Proof.
   intros nm. destruct s; simpl; intros h; try discriminate.
   - myInjection h. reflexivity.
@@ -736,7 +741,7 @@ Qed.
 
 Lemma Fix_strip_inv:
   forall ds n s, TFix ds n = strip s ->
-    exists sds, (L1g.compile.TFix sds n) = s /\ ds = stripDs sds.
+    exists sds, (L2.compile.TFix sds n) = s /\ ds = stripDs sds.
 Proof.
   intros ds n. destruct s; simpl; intros h; try discriminate.
   - myInjection h. exists d. intuition.
@@ -745,7 +750,7 @@ Qed.
 Lemma App_strip_inv:
   forall fn arg args s, TApp fn arg args = strip s ->
     exists sfn sarg sargs,
-      (L1g.compile.TApp sfn sarg sargs) = s /\
+      (L2.compile.TApp sfn sarg sargs) = s /\
       fn = strip sfn /\ arg = strip sarg /\ args = strips sargs.
 Proof.
   intros fn arg args. destruct s; simpl; intros h; try discriminate.
@@ -755,7 +760,7 @@ Qed.
 Lemma LetIn_strip_inv:
   forall nm dfn bod s, TLetIn nm dfn bod = strip s ->
     exists sdfn sty sbod,
-      (L1g.compile.TLetIn nm sdfn sty sbod = s) /\
+      (L2.compile.TLetIn nm sdfn sty sbod = s) /\
       dfn = strip sdfn /\ bod = strip sbod.
 Proof.
   intros nm dfn bod s. destruct s; simpl; intros h; try discriminate.
@@ -764,7 +769,7 @@ Qed.
 
 Lemma Case_strip_inv:
   forall m mch brs s, TCase m mch brs = strip s ->
-    exists sty smch sbrs, (L1g.compile.TCase m sty smch sbrs = s) /\
+    exists sty smch sbrs, (L2.compile.TCase m sty smch sbrs = s) /\
               mch = strip smch /\ brs = stripDs sbrs.
 Proof.
   intros m mch brs s. destruct s; simpl; intros h; try discriminate.
@@ -772,7 +777,7 @@ Proof.
 Qed.
 
 Lemma tnil_strip_inv:
-  forall ts, tnil = strips ts -> ts = L1g.compile.tnil.
+  forall ts, tnil = strips ts -> ts = L2.compile.tnil.
 Proof.
   induction ts; intros; try reflexivity.
   - simpl in H. discriminate.
@@ -780,7 +785,7 @@ Qed.
 
 Lemma tcons_strip_inv:
   forall t ts us, tcons t ts = strips us ->
-    exists st sts, (L1g.compile.tcons st sts = us) /\ 
+    exists st sts, (L2.compile.tcons st sts = us) /\ 
                    t = strip st /\ ts = strips sts.
 Proof.
   intros t ts us. destruct us; simpl; intros h; try discriminate.
@@ -789,7 +794,7 @@ Qed.
 
 Lemma dcons_strip_inv:
   forall nm t m ts us, dcons nm t m ts = stripDs us ->
-    exists ty st sts, (L1g.compile.dcons nm ty st m sts = us) /\ 
+    exists ty st sts, (L2.compile.dcons nm ty st m sts = us) /\ 
                    t = strip st /\ ts = stripDs sts.
 Proof.
   intros nm t m ts us. destruct us; simpl; intros h; try discriminate.
@@ -798,93 +803,54 @@ Qed.
 
 Lemma whCaseStep_Hom:
   forall n ts bs t,
-    L1g.term.whCaseStep n ts bs = Some t -> 
+    L2.term.whCaseStep n ts bs = Some t -> 
     whCaseStep n (strips ts) (stripDs bs) = Some (strip t).
 Proof.
   intros n ts bs t h. rewrite <- whCaseStep_hom. rewrite <- optStrip_hom.
   apply f_equal. assumption.
 Qed.
 
-Definition excStrip (t:exception L1gTerm) : exception Term :=
+Definition excStrip (t:exception L2Term) : exception Term :=
   match t with
     | Exc str => Exc str
     | Ret t => Ret (strip t)
   end.
 
 
-Theorem L2WcbvEval_sound_for_L1gWcbvEval:
-  forall (p:environ L1g.compile.Term) (t:L1g.compile.Term) (L2s:Term),
+Theorem L2WcbvEval_sound_for_L2WcbvEval:
+  forall (p:environ L2.compile.Term) (t:L2.compile.Term) (L2s:Term),
     WcbvEval (stripEnv p) (strip t) L2s ->
-  forall s, L1g.wcbvEval.WcbvEval p t s -> L2s = strip s.
+  forall s, L2.wcbvEval.WcbvEval p t s -> L2s = strip s.
 Proof.
   intros. refine (WcbvEval_single_valued _ _).
   - eassumption.
   - apply WcbvEval_hom. assumption.
 Qed.
-Print Assumptions L2WcbvEval_sound_for_L1gWcbvEval.
-
-(******
-Theorem L2WcbvEval_sound_for_L1gwndEval:
-  forall p t s, WcbvEval (stripEnv p) (strip t) (strip s) ->
-           L1g.program.WFaEnv p -> L1g.term.WFapp t ->        
-        L1g.wndEval.wndEvalRTC p t s.
-Proof.
-  intros.
-  refine (proj1 (L1g.wcbvEval.WcbvEval_wndEvalRTC _) _ _ _ _);
-    try assumption.
-  
-Qed.
-Print Assumptions L2WcbvEval_sound_for_L1gwndEval.
- *****************)
-
-Theorem L2WcbvEval_sound_for_L1gwndEval:
-  forall (p:environ L1g.compile.Term) (t:L1g.compile.Term) (L2s:Term),
-    WcbvEval (stripEnv p) (strip t) L2s ->
-    forall s, L1g.wcbvEval.WcbvEval p t s ->
-              L1g.program.WFaEnv p -> L1g.term.WFapp t ->        
-              L1g.wndEval.wndEvalRTC p t s.
-Proof.
-  intros.
-  refine (proj1 (L1g.wcbvEval.WcbvEval_wndEvalRTC _) _ _ _ _); assumption.
-Qed.
-Print Assumptions L2WcbvEval_sound_for_L1gwndEval.
-
-(*****
-Parameter ObsCrct: Term -> L1g.compile.Term -> Prop.
-Goal
-  forall (sp:environ L1g.compile.Term) (st:L1g.compile.Term),
-   (exists ou:Term, WcbvEval (stripEnv sp) (strip st) ou ->
-       exists su, L1g.wcbvEval.WcbvEval sp st su /\ ObsCrct ou su) /\
-(forall (su:L1g.compile.Term),
-  L1g.wcbvEval.WcbvEval sp st su ->
-    exists ou:Term, WcbvEval (stripEnv sp) (strip st) ou).
-Proof.
-  split; intros. Focus 2.
-*******************)
-  
+Print Assumptions L2WcbvEval_sound_for_L2WcbvEval.
 
 
-    
 Lemma sound_and_complete:
-  forall (p:environ L1g.compile.Term) (t s:L1g.compile.Term),
-    L1g.wcbvEval.WcbvEval p t s ->
+  forall (p:environ L2.compile.Term) (t s:L2.compile.Term),
+    L2.wcbvEval.WcbvEval p t s ->
     WcbvEval (stripEnv p) (strip t) (strip s).
 Proof.
   intros p t s h. apply (proj1 (WcbvEval_hom p)). assumption.
 Qed.
 
 Lemma sac_complete:
-  forall p t s, L1g.wcbvEval.WcbvEval p t s ->
+  forall p t s, L2.wcbvEval.WcbvEval p t s ->
                 WcbvEval (stripEnv p) (strip t) (strip s).
 Proof.
   intros. apply sound_and_complete. assumption.
 Qed.
 
 Lemma sac_sound:
-  forall p t s, L1g.wcbvEval.WcbvEval p t s ->
+  forall p t s, L2.wcbvEval.WcbvEval p t s ->
   forall L2s, WcbvEval (stripEnv p) (strip t) L2s -> L2s = strip s.
 Proof.
   intros p t s h1 L2s h2.
   apply (WcbvEval_single_valued h2). apply (sound_and_complete h1).
 Qed. 
 Print Assumptions sac_sound.
+
+*******************************)
