theories/L2_5_box/instances.v
@@ -1,5 +1,5 @@
+
 Require Import L2_5.compile.
-(* Require Import L2.wcbvEval. *)
 Require Import certiClasses.
 Require Import Common.Common.
 
@@ -26,11 +26,6 @@ Instance certiL2_5 : CerticoqLanguage (Program L2_5.compile.Term) := {}.
 
 
 Instance certiL2_to_L2_5: 
-  CerticoqTotalTranslation (Program L2.compile.Term) (Program L2_5.compile.Term) :=
-L2_5.compile.L2Pgm_Program.
-
-
-
-
-
-
+  CerticoqTotalTranslation (Program L2k.compile.Term)
+                           (Program L2_5.compile.Term) :=
+  L2_5.compile.L2kPgm_Program.
